compiler/dafny/semantics/dafny_evaluatePropsScript.sml
@@ -55,6 +55,7 @@ Proof
   \\ gvs [evaluate_exp_def, unuse_old_def, use_old_def, restore_caller_def,
           unuse_prev_def, use_prev_def, unset_prev_def, set_prev_def,
           unuse_prev_heap_def, use_prev_heap_def,
+          unuse_old_heap_def, use_old_heap_def,
           set_up_call_def, dec_clock_def, AllCaseEqs()]
   \\ simp [state_component_equality]
 QED
@@ -275,6 +276,8 @@ Proof
          dec_clock_def, AllCaseEqs()])
   >~ [‘Old’] >-
    (gvs [evaluate_exp_def, use_old_def, unuse_old_def, AllCaseEqs()])
+  >~ [‘OldHeap’] >-
+   (gvs [evaluate_exp_def, use_old_heap_def, unuse_old_heap_def, AllCaseEqs()])
   >~ [‘Prev’] >-
    (gvs [evaluate_exp_def, use_prev_def, unuse_prev_def, AllCaseEqs()])
   >~ [‘PrevHeap’] >-
