compiler/dafny/semantics/dafny_evaluateScript.sml
@@ -113,6 +113,10 @@ Definition evaluate_exp_ann_def[nocompute]:
   (if env.is_running then (st, Rerr Rtype_error) else
    (case evaluate_exp (use_old st) env e of
     | (st₁, r) => (unuse_old st₁ st, r))) ∧
+  evaluate_exp st env (OldHeap e) =
+  (if env.is_running then (st, Rerr Rtype_error) else
+   (case evaluate_exp (use_old_heap st) env e of
+    | (st₁, r) => (unuse_old_heap st₁ st, r))) ∧
   evaluate_exp st env (Prev e) =
   (if env.is_running then (st, Rerr Rtype_error) else
    (case evaluate_exp (use_prev st) env e of
@@ -170,6 +174,7 @@ Termination
           push_locals_def, use_old_def, unuse_old_def, oneline do_cond_def,
           use_prev_def, unuse_prev_def, set_prev_def, unset_prev_def,
           use_prev_heap_def, unuse_prev_heap_def,
+          use_old_heap_def, unuse_old_heap_def,
           UNZIP_MAP, list_size_pair_size_MAP_FST_SND, AllCaseEqs ()]
 End
 
@@ -189,6 +194,7 @@ Proof
           push_locals_def, pop_locals_def,
           use_prev_def, unuse_prev_def, set_prev_def, unset_prev_def,
           use_prev_heap_def, unuse_prev_heap_def,
+          use_old_heap_def, unuse_old_heap_def,
           use_old_def, unuse_old_def, evaluate_exp_ann_def, AllCaseEqs ()]
   \\ EVERY (map imp_res_tac
                 [set_up_call_clock_eq, restore_caller_clock, fix_clock_IMP])
